\documentclass[
a4paper,
10pt,
twoside,
% prd,
% aps,
% nofootinbib,
% superscriptaddress,
% floatfix,
% preprintnumbers,
]{article}

% MUST BE RUN WITH LUALATEXMK

\usepackage{preamble}
\usepackage{titleinfo}

\geometry{ % Set document margins
	top			= 2cm,
	bottom		= 2cm,
	left		= 1cm,
	right		= 1cm
}

\newcommand{\mcols}{2} % Choose number of columns (>= 1)


\bibSetup{refs.bib} % Give references file 
% ===== Format headers & footers =====

\pagestyle{fancy}
\fancyhf{}
\fancyhead[LE,RO]{B. Henke}
\fancyhead[LO]{\headertitle\hspace{0.5cm}\textit{PHY981}}
\fancyhead[RE]{\textit{PHY981}\hspace{0.5cm}\headertitle}
\fancyfoot[RE,LO]{\thepage}

\begin{document}
% \tableofcontents
\titleinf{Lipkin Model}
\maketitle
\startmcols

\section{Introduction}\label{sec: I}

Consider a two level system with the lower energy state ($\sigma = -1$) having an energy of $-\epsilon/2$ and the upper energy state ($\sigma=1$) having an energy of $\epsilon/2$.
Now, consider a another system with $\Omega \in \Z^+$ copies of this two level system.

This gives a system with two quantum numbers, $\sigma \in \{-1,1\}$, and $m \in \{1,2,\dots,\Omega\}$.
In Fock space, the Hamiltonian for this system is
\begin{align}
	\hat{H} &= \frac{1}{2} \epsilon \sum_{m\sigma}\sigma a_{m\sigma}^\dagger a_{m\sigma}- \frac{1}{2}V\sum_{mm'\sigma}a_{m\sigma}^\dagger a_{m'\sigma}^\dagger a_{m'-\sigma}a_{m-\sigma}.
	\label{eq: lipkin_ham_a}
\end{align}
The $V$ term here is the two particle interaction term between adjacent particles.

\subsection{Quasi-spin Operators} \label{ssec: IA}

One can consider the operators
\begin{align}
	\hat{K}_3 &= \frac{1}{2} \sum_{m=1}^\Omega (a_{m+}^\dagger a_{m+}-a_{m-}^\dagger a_{m-}),\\
	\hat{K}_+ &= \sum_{m=1}^\Omega a_{m+}^\dagger a_{m-},\\
	\hat{K}_- &= (\hat{K}_+)^\dagger,\\
		&= \sum_{m=1}^\Omega a_{m-}^\dagger a_{m+}.
\end{align}

Using these "quasi-spin" operators, one can write \ref{eq: lipkin_ham_a} as
\begin{align}
	\hat{H} &= \epsilon \hat{K}_3 - \frac{1}{2}V (\hat{K}_+^2-\hat{K}_-^2).
	\label{eq: lipkin_ham_k}
\end{align}


\subsubsection{Commutation Relations} \label{sssec: IA1}

\begin{align}
	[\hat{K}_+,\hat{K}_-]
		&= \sum_{m=1}^\Omega\sum_{n=1}^\Omega a_{m+}^\dagger a_{m-} a_{n-}^\dagger a_{n+} - a_{n-}^\dagger a_{n+} a_{m+}^\dagger a_{m-},\\
		&= \sum_{m=1}^\Omega\sum_{n=1}^\Omega a_{m+}^\dagger (\delta_{m-n-} - a_{n-}^\dagger a_{m-}) a_{n+}\nonumber\\
		&- \sum_{m=1}^\Omega\sum_{n=1}^\Omega a_{n-}^\dagger (\delta_{m+n+} - a_{m+}^\dagger a_{n+}) a_{m-},\\
		&= \sum_{m=1}^\Omega a_{m+}^\dagger a_{m+} - a_{m-}^\dagger a_{m-}\nonumber\\
		&+ \sum_{m=1}^\Omega\sum_{n=1}^\Omega a_{n-}^\dagger a_{m+}^\dagger a_{n+} a_{m-} - a_{m+}^\dagger a_{n-}^\dagger a_{m-} a_{n+},\\
		&= 2\hat{K}_3 + 0,\\
		&= 2\hat{K}_3.
\end{align}

\begin{align}
	[\hat{K}_3,\hat{K}_\pm]
		&= \frac{1}{2} \sum_{m=1}^\Omega\sum_{n=1}^\Omega (a_{m+}^\dagger a_{m+}-a_{m-}^\dagger a_{m-}) a_{n\pm}^\dagger a_{n\mp} \nonumber\\
		&- \frac{1}{2} \sum_{m=1}^\Omega\sum_{n=1}^\Omega a_{n\pm}^\dagger a_{n\mp} (a_{m+}^\dagger a_{m+}-a_{m-}^\dagger a_{m-}),\\
		&= \frac{1}{2} \sum_{m=1}^\Omega\sum_{n=1}^\Omega (a_{m+}^\dagger a_{m+} a_{n\pm}^\dagger a_{n\mp} - a_{m-}^\dagger a_{m-} a_{n\pm}^\dagger a_{n\mp}) \nonumber\\
		&- \frac{1}{2} \sum_{m=1}^\Omega\sum_{n=1}^\Omega (a_{n\pm}^\dagger a_{n\mp} a_{m+}^\dagger a_{m+} - a_{n\pm}^\dagger a_{n\mp} a_{m-}^\dagger a_{m-})\\
		&= \frac{1}{2} \sum_{m=1}^\Omega\sum_{n=1}^\Omega (a_{m+}^\dagger \delta_{m+n\pm} a_{n\mp} - a_{m-}^\dagger \delta_{m-n\pm} a_{n\mp} \nonumber\\
		&\qquad - a_{m+}^\dagger a_{n\pm}^\dagger a_{m+} a_{n\mp} + a_{m-}^\dagger a_{n\pm}^\dagger a_{m-} a_{n\mp}) \nonumber\\
		&- \frac{1}{2} \sum_{m=1}^\Omega\sum_{n=1}^\Omega (a_{n\pm}^\dagger \delta_{n\mp m+} a_{m+} - a_{n\pm}^\dagger \delta_{n\mp m-}a_{m-} \nonumber\\
		&\qquad - a_{n\pm}^\dagger a_{m+}^\dagger a_{n\mp} a_{m+} + a_{n\pm}^\dagger a_{m-}^\dagger a_{n\mp} a_{m-}),\\
		&= \sum_{m=1}^\Omega (a_{m+}^\dagger a_{m-} - a_{m-}^\dagger a_{m+}) \nonumber\\
		&+ \frac{1}{2} \sum_{m=1}^\Omega\sum_{n=1}^\Omega (a_{m-}^\dagger a_{n\pm}^\dagger a_{m-} a_{n\mp} - a_{m+}^\dagger a_{n\pm}^\dagger a_{m+} a_{n\mp}) \nonumber\\
		&+ \frac{1}{2} \sum_{m=1}^\Omega\sum_{n=1}^\Omega (a_{n\pm}^\dagger a_{m+}^\dagger a_{n\mp} a_{m+} - a_{n\pm}^\dagger a_{m-}^\dagger a_{n\mp} a_{m-}),
\end{align}

% \printbib
\stopmcols

\end{document}